Cslib/Computability/Machines/Turing/MultiTape/Combinators/Ite.lean
@@ -9,7 +9,6 @@ module
 public import Cslib.Computability.Machines.Turing.MultiTape.Combinators.Comp
 public import Cslib.Computability.Machines.Turing.MultiTape.Combinators.AlmostConstant
 public import Cslib.Computability.Machines.Turing.MultiTape.Plumbing.Branch
-public import Cslib.Computability.Machines.Turing.MultiTape.Plumbing.InputBranch
 public import Cslib.Computability.Machines.Turing.MultiTape.NormalForms.Adapters
 public import Cslib.Computability.Machines.Turing.MultiTape.Combinators.Concat
 public import Cslib.Computability.Machines.Turing.MultiTape.Combinators.TakeDrop
